Progress through concurrent file_get_attr_ok proof

src/ConcurrentFS.v
@@ -9,52 +9,74 @@ Import Log FSLayout Inode.INODE BFile.
 Import BFILE.
 Import SuperBlock.
 Import GenSepN.
+Import Pred.
 
 Require Import HomeDirProtocol.
-
-Record FSParams St :=
-  { fs_cache : CacheParams St;
-    fsmem: var (Mem St) memstate;
-    fstree: var (Abstraction St) dirtree;
-    (* static configurations: *)
-    homedirs: TID -> list string;
-    fsparams: fs_xparams; }.
-
-Definition fs_invariant St (FP: FSParams St) sigma :=
-    let tree := get_var (fstree FP) (Sigma.s sigma) in
-    let fsxp := fsparams FP in
-    let mscs := get_var (fsmem FP) (Sigma.mem sigma) in
-    let CP := fs_cache FP in
-    exists ds ilist frees,
-      LOG.rep (FSLayout.FSXPLog fsxp) (SB.rep fsxp)
-              (LOG.NoTxn ds) (MSLL mscs) (Sigma.hm sigma)
-              (seq_disk CP sigma) /\
-      (DirTreeRep.rep fsxp Pred.emp tree ilist frees)
-        (list2nmem (ds!!)).
-
-Definition fs_guarantee St (FP: FSParams St) tid sigma sigma' :=
-    CacheRep (fs_cache FP) empty_writebuffer sigma /\
-    CacheRep (fs_cache FP) empty_writebuffer sigma' /\
-    fs_invariant FP sigma /\
-    fs_invariant FP sigma' /\
-    let tree := get_var (fstree FP) (Sigma.s sigma) in
-    let tree' := get_var (fstree FP) (Sigma.s sigma') in
-    homedir_guarantee tid (homedirs FP) tree tree'.
+Require Import RelationClasses.
 
 Section ConcurrentFS.
 
-  Context {St:StateTypes}.
-  Variable G:Protocol St.
-  Variable FP:FSParams St.
-  Variable fsG: forall tid sigma sigma',
-      G tid sigma sigma ->
-      fs_guarantee FP tid sigma sigma'.
+  Context {OtherSt:StateTypes}.
 
-  Definition get_fsmem := get_var (fsmem FP).
-  Definition set_fsmem := set_var (fsmem FP).
-  Definition upd_fstree s update := set_var (fstree FP) s (update (get_var (fstree FP) s)).
+  Record FsMem :=
+    fsMem { fsmem: memstate;
+            fs_other_mem: Mem OtherSt; }.
 
-  Definition fsxp := fsparams FP.
+  Record FsAbstraction :=
+    fsAbstraction { fstree: dirtree;
+                    homedirs: TID -> list string;
+                    fs_other_s : Abstraction OtherSt; }.
+
+  Definition St := OptimisticCache.St
+                     {| Mem := FsMem;
+                        Abstraction := FsAbstraction; |}.
+
+  Variable fsxp: fs_xparams.
+
+  Definition get_fsmem (m: Mem St) :=
+    fsmem (cache_other_mem m).
+  Definition get_fstree (sigma: Sigma St) :=
+    fstree (cache_other_s (Sigma.s sigma)).
+  Definition get_homedirs (sigma: Sigma St) :=
+    homedirs (cache_other_s (Sigma.s sigma)).
+
+  Definition fs_invariant wb (sigma: Sigma St) :=
+    let tree := get_fstree sigma in
+    let mscs := get_fsmem (Sigma.mem sigma) in
+    CacheRep wb sigma /\
+    exists ds ilist frees,
+      LOG.rep (FSLayout.FSXPLog fsxp) (SB.rep fsxp)
+              (LOG.NoTxn ds) (MSLL mscs) (Sigma.hm sigma)
+              (seq_disk sigma) /\
+      (DirTreeRep.rep fsxp Pred.emp tree ilist frees)
+        (list2nmem (ds!!)).
+
+  Definition fs_guarantee' wb' tid (sigma sigma':Sigma St) :=
+    fs_invariant empty_writebuffer sigma /\
+    fs_invariant wb' sigma' /\
+    let tree := get_fstree sigma in
+    let tree' := get_fstree sigma' in
+    homedir_guarantee tid (get_homedirs sigma) tree tree' /\
+    get_homedirs sigma' = get_homedirs sigma.
+
+  Definition fs_guarantee :=
+    fs_guarantee' empty_writebuffer.
+
+  (* TODO: eventually abstract away protocol *)
+
+  (* TODO: provide mem/abstraction setter/updater in cache, and here: callers
+  should not have to deal with listing out the other parts of these records *)
+
+  Definition set_fsmem (m: Mem St) fsm : Mem St :=
+    let other := fs_other_mem (cache_other_mem m) in
+    cacheMem (St:={|Mem:=FsMem|}) (cache m)
+             (fsMem fsm other).
+
+  Definition upd_fstree update (s: Abstraction St) : Abstraction St :=
+    let fsS0 := cache_other_s s in
+    let other := fs_other_s fsS0 in
+    cacheS (St:={|Abstraction:=FsAbstraction|}) (vdisk_committed s) (vdisk s)
+           (fsAbstraction (update (fstree fsS0)) (homedirs fsS0) other).
 
   Definition guard {T} (r: Result T) : {exists v, r=Success v} + {r=Failed}.
     destruct r; eauto.
@@ -62,27 +84,186 @@ Section ConcurrentFS.
 
   Definition retry_syscall T
              (p: memstate -> @cprog St (Result (memstate * T) * WriteBuffer))
-             (update: TID -> dirtree -> dirtree)
+             (update: dirtree -> dirtree)
     : cprog (Result T) :=
     retry guard (m <- Get;
                    do '(r, wb) <- p (get_fsmem m);
                    match r with
                    | Success (ms', r) =>
-                     _ <- CacheCommit (fs_cache FP) wb;
+                     _ <- CacheCommit wb;
                        m <- Get;
                        _ <- Assgn (set_fsmem m ms');
-                       _ <- GhostUpdate (fun tid s => upd_fstree s (update tid));
+                       _ <- GhostUpdate (fun _ s => upd_fstree update s);
                        Ret (Success r)
                    | Failed =>
-                     _ <- CacheAbort (fs_cache FP) wb;
+                     _ <- CacheAbort;
                        _ <- Yield;
                        Ret Failed
                    end).
 
-  Definition file_get_attr inum :=
+  Definition file_get_attr inum : @cprog St _ :=
     retry_syscall (fun mscs =>
-                     OptFS.file_get_attr (fs_cache FP) fsxp inum mscs empty_writebuffer)
-                  (fun _ => id).
+                     OptFS.file_get_attr _ fsxp inum mscs empty_writebuffer)
+                  (fun tree => tree).
+
+  Lemma exists_tuple : forall A B P,
+      (exists a b, P (a, b)) ->
+      exists (a: A * B), P a.
+  Proof.
+    intros.
+    repeat deex; eauto.
+  Qed.
+
+  Ltac split_lift_prop :=
+    unfold Prog.pair_args_helper in *; simpl in *;
+    repeat match goal with
+           | [ H: context[(emp * _)%pred] |- _ ] =>
+             apply star_emp_pimpl in H
+           | [ H: context[(_ * [[ _ ]])%pred] |- _ ] =>
+             apply sep_star_lift_apply in H
+           | [ H : _ /\ _ |- _ ] => destruct H
+           | _ => progress subst
+           end.
+
+  Section GetAttrCleanSpec.
+
+    Hint Extern 0 {{ OptFS.file_get_attr _ _ _ _ _; _ }} => apply OptFS.file_get_attr_ok : prog.
+
+    Theorem file_get_attr1_ok : forall inum tid mscs,
+        cprog_spec fs_guarantee tid
+                   (fun '(pathname, f) '(sigma_i, sigma) =>
+                      {| precondition :=
+                           fs_guarantee tid sigma_i sigma /\
+                           mscs = get_fsmem (Sigma.mem sigma) /\
+                           let tree := get_fstree sigma in
+                           find_subtree pathname tree = Some (TreeFile inum f);
+                         postcondition :=
+                           fun '(sigma_i', sigma') '(r, wb') =>
+                             get_fstree sigma' = get_fstree sigma /\
+                             match r with
+                             | Success (mscs', (r, _)) =>
+                               r = BFILE.BFAttr f /\
+                               fs_guarantee' wb' tid sigma_i'
+                                             (Sigma.set_mem sigma' (set_fsmem (Sigma.mem sigma') mscs'))
+                             | Failed =>
+                               fs_guarantee' wb' tid sigma_i' sigma'
+                             end
+                      |}) (OptFS.file_get_attr _ fsxp inum mscs empty_writebuffer).
+    Proof.
+      intros.
+      step.
+
+      unfold OptFS.framed_spec, translate_spec; simpl.
+      repeat apply exists_tuple; simpl.
+      unfold fs_guarantee, fs_guarantee', fs_invariant in *; intuition;
+        repeat deex.
+
+      repeat eexists.
+      SepAuto.pred_apply; SepAuto.cancel; eauto.
+      apply H3. (* why is CacheRep getting unfolded? *)
+      apply H3.
+
+      intros.
+      step.
+      destruct r; intuition eauto.
+
+
+      unfold get_fstree, locally_modified in *; fold St in *; intuition eauto.
+      congruence.
+
+      destruct r; intuition eauto.
+      split_lift_prop; auto.
+      destruct v.
+      destruct p; simpl in *; subst; intuition eauto.
+
+      unfold CacheRep in *; destruct sigma, sigma'; simpl in *; intuition eauto.
+
+      unfold get_fstree, locally_modified in *; simpl in *; eauto.
+      destruct sigma, sigma'; simpl in *; auto.
+
+      exists ds, ilist, frees.
+      repeat match goal with
+             | [ |- exists _, _ ] => eexists
+             end; intuition eauto.
+      congruence.
+
+      unfold get_fstree, locally_modified in *.
+      destruct sigma, sigma' in *; simpl in *; intuition eauto.
+      etransitivity; eauto.
+      match goal with
+      | [ |- homedir_guarantee _ _ ?tree ?tree' ] =>
+        replace tree' with tree by congruence
+      end; reflexivity.
+
+      unfold get_homedirs, set_fsmem, get_fstree, locally_modified in *.
+      destruct sigma_i, sigma, sigma' in *; simpl in *; intuition.
+      congruence.
+
+      subst; eauto.
+      (* TODO: much duplication with above, most likely *)
+    Admitted.
+
+  End GetAttrCleanSpec.
+
+  Hint Extern 0 {{ OptFS.file_get_attr _ _ _ _ _; _ }} => apply file_get_attr1_ok : prog.
+
+  Hint Extern 0 {{ CacheCommit _; _ }} => apply CacheCommit_ok : prog.
+  Hint Extern 0 {{ CacheAbort; _ }} => apply CacheAbort_ok : prog.
+
+  Theorem file_get_attr_ok : forall inum tid,
+      cprog_spec fs_guarantee tid
+                 (fun '(pathname, f) '(sigma_i, sigma) =>
+                    {| precondition :=
+                         fs_guarantee tid sigma_i sigma /\
+                         let tree := get_fstree sigma in
+                         find_subtree pathname tree = Some (TreeFile inum f);
+                       postcondition :=
+                         fun '(sigma_i', sigma') r =>
+                           Rely fs_guarantee tid sigma sigma' /\
+                           get_fstree sigma' = get_fstree sigma /\
+                           match r with
+                           | Success (r, _) => r = BFILE.BFAttr f
+                           | Failed => True
+                           end
+                    |}) (file_get_attr inum).
+  Proof.
+    unfold file_get_attr, retry_syscall; intros.
+
+    eapply retry_spec'; induction n; simpl.
+    - step.
+      step.
+
+      apply exists_tuple; do 2 eexists; simpl; intuition eauto.
+
+      destruct a.
+      destruct v.
+      step.
+
+      destruct p; intuition eauto.
+      subst.
+      unfold fs_guarantee', fs_invariant in H5; intuition eauto.
+      destruct sigma'; simpl in *; eauto.
+
+      step.
+      step.
+      step.
+      step.
+      intuition eauto.
+
+      admit. (* rely holds, despite storing new mscs *)
+
+      fold St in *.
+      unfold get_fstree, locally_modified, id in *.
+      destruct sigma, sigma', sigma0; simpl in *; intuition.
+      congruence.
+
+      step.
+      unfold fs_guarantee', fs_invariant in *; intuition eauto; repeat deex.
+      eexists; intuition eauto.
+
+      step.
+      intuition eauto.
+  Abort.
 
 End ConcurrentFS.
 
